Added programs with specs for the coexponential protocols

theories/channel/exponentials.v
@@ -1,5 +1,5 @@
-From actris.channel Require Import channel.
-From actris.channel Require Import proofmode.
+From actris.channel Require Import channel proofmode.
+From iris.heap_lang.lib Require Import par.
 
 (**
 Inspired by the work of Qian et al.
@@ -16,56 +16,64 @@ S ⨁ T   = S <+> T
 S & T   = S <&> T
 *)
 
-Section exponentials.
+Section exponential_prot.
   Context `{heapG Σ, chanG Σ}.
 
   (** F_A(X) ≜ 1 & A & (X ⨂ X) *)
-  Definition of_course_aux (A : iProto Σ) (rec : iProto Σ) : iProto Σ :=
+  Definition iProto_of_course_aux (A : iProto Σ) (rec : iProto Σ) : iProto Σ :=
     (END <&> (A <&> (<!(c:val)> MSG c {{ c ↣ rec }}; rec)))%proto.
-  Instance of_course_aux_contractive A : Contractive (of_course_aux A).
+  Instance iProto_of_course_aux_contractive A : Contractive (iProto_of_course_aux A).
   Proof. solve_proto_contractive. Qed.
   (** !A ≜ ν X. F_A(X) *)
-  Definition of_course (A : iProto Σ) : iProto Σ := fixpoint (of_course_aux A).
-  Lemma of_course_unfold A : of_course A ≡ of_course_aux A (of_course A).
-  Proof. by rewrite /of_course {1}(fixpoint_unfold (of_course_aux A)). Qed.
+  Definition iProto_of_course (A : iProto Σ) : iProto Σ :=
+    fixpoint (iProto_of_course_aux A).
+  Lemma iProto_of_course_unfold A :
+    iProto_of_course A ≡ iProto_of_course_aux A (iProto_of_course A).
+  Proof.
+      by rewrite /iProto_of_course
+                 {1}(fixpoint_unfold (iProto_of_course_aux A)).
+  Qed.
 
   (** G_A(X) ≜ ⊥ ⨁ A ⨁ (X _&_ X) *)
-  Definition why_not_aux (A : iProto Σ) (rec : iProto Σ) : iProto Σ :=
+  Definition iProto_why_not_aux (A : iProto Σ) (rec : iProto Σ) : iProto Σ :=
     (END <+> (A <+> (<?(c:val)> MSG c {{ c ↣ iProto_dual rec }}; rec)))%proto.
-  Instance why_not_aux_contractive A : Contractive (why_not_aux A).
+  Instance iProto_why_not_aux_contractive A : Contractive (iProto_why_not_aux A).
   Proof. solve_proto_contractive. Qed.
   (** ?A ≜  μ X. G_A(X) *)
-  Definition why_not (A : iProto Σ) := fixpoint (why_not_aux A).
-  Lemma why_not_unfold A : why_not A ≡ why_not_aux A (why_not A).
-  Proof. by rewrite /why_not {1}(fixpoint_unfold (why_not_aux A)). Qed.
+  Definition iProto_why_not (A : iProto Σ) := fixpoint (iProto_why_not_aux A).
+  Lemma iProto_why_not_unfold A :
+    iProto_why_not A ≡ iProto_why_not_aux A (iProto_why_not A).
+  Proof. by rewrite /iProto_why_not {1}(fixpoint_unfold (iProto_why_not_aux A)). Qed.
 
   (** H_A(X) ≜ ⊥ & A & (X _&_ X) *)
-  Definition server_aux (A : iProto Σ) (rec : iProto Σ) : iProto Σ :=
+  Definition iProto_server_aux (A : iProto Σ) (rec : iProto Σ) : iProto Σ :=
     (END <&> (A <&> (<?(c:val)> MSG c {{ c ↣ rec }}; rec)))%proto.
-  Instance server_aux_contractive A : Contractive (server_aux A).
+  Instance iProto_server_aux_contractive A : Contractive (iProto_server_aux A).
   Proof. solve_proto_contractive. Qed.
   (** _!_A ≜ μ X. H_A(X) *)
-  Definition server (A : iProto Σ) := fixpoint (server_aux A).
-  Lemma server_unfold A : server A ≡ server_aux A (server A).
-  Proof. by rewrite /server {1}(fixpoint_unfold (server_aux A)). Qed.
+  Definition iProto_server (A : iProto Σ) := fixpoint (iProto_server_aux A).
+  Lemma iProto_server_unfold A :
+    iProto_server A ≡ iProto_server_aux A (iProto_server A).
+  Proof. by rewrite /iProto_server {1}(fixpoint_unfold (iProto_server_aux A)). Qed.
 
   (** K_A(X) ≜ 1 ⨁ A ⨁ (X ⨂ X) *)
-  Definition client_aux (A : iProto Σ) (rec : iProto Σ) : iProto Σ :=
+  Definition iProto_client_aux (A : iProto Σ) (rec : iProto Σ) : iProto Σ :=
     (END <+> (A <+> (<!(c:val)> MSG c {{ c ↣ iProto_dual rec }}; rec)))%proto.
-  Instance client_aux_contractive A : Contractive (client_aux A).
+  Instance iProto_client_aux_contractive A : Contractive (iProto_client_aux A).
   Proof. solve_proto_contractive. Qed.
   (** _?_A ≜ μ X. K_A(X) *)
-  Definition client (A : iProto Σ) := fixpoint (client_aux A).
-  Lemma client_unfold A : client A ≡ client_aux A (client A).
-  Proof. by rewrite /client {1}(fixpoint_unfold (client_aux A)). Qed.
+  Definition iProto_client (A : iProto Σ) := fixpoint (iProto_client_aux A).
+  Lemma iProto_client_unfold A :
+    iProto_client A ≡ iProto_client_aux A (iProto_client A).
+  Proof. by rewrite /iProto_client {1}(fixpoint_unfold (iProto_client_aux A)). Qed.
 
   (** (?A)^⟂ = !(A^⟂)*)
   Lemma why_not_of_course_dual (A : iProto Σ) :
-    iProto_dual (why_not A) ≡ of_course (iProto_dual A).
+    iProto_dual (iProto_why_not A) ≡ iProto_of_course (iProto_dual A).
   Proof.
     apply (uPred.internal_eq_soundness (M:=iResUR Σ)).
     iLöb as "IH" forall (A).
-    iEval (rewrite why_not_unfold of_course_unfold).
+    iEval (rewrite iProto_why_not_unfold iProto_of_course_unfold).
     rewrite iProto_dual_choice iProto_dual_end.
     iApply iProto_choice_equiv; repeat iSplit; try done.
     rewrite iProto_dual_choice.
@@ -97,11 +105,11 @@ Section exponentials.
 
   (** (_?_A)^⟂ = _!_(A^⟂)*)
   Lemma client_server_dual (A : iProto Σ) :
-    iProto_dual (client A) ≡ server (iProto_dual A).
+    iProto_dual (iProto_client A) ≡ iProto_server (iProto_dual A).
   Proof.
     apply (uPred.internal_eq_soundness (M:=iResUR Σ)).
     iLöb as "IH" forall (A).
-    iEval (rewrite client_unfold server_unfold).
+    iEval (rewrite iProto_client_unfold iProto_server_unfold).
     rewrite iProto_dual_choice iProto_dual_end.
     iApply iProto_choice_equiv; repeat iSplit; try done.
     rewrite iProto_dual_choice.
@@ -131,4 +139,83 @@ Section exponentials.
       by iFrame.
   Qed.
 
-End exponentials.
+End exponential_prot.
+
+Notation "<|¡|> A" := (iProto_server A) (at level 100) : proto_scope.
+Notation "<|¿|> A" := (iProto_client A) (at level 100) : proto_scope.
+Notation "<|!|> A" := (iProto_of_course A) (at level 100) : proto_scope.
+Notation "<|?|> A" := (iProto_why_not A) (at level 100) : proto_scope.
+
+Definition server : val :=
+  rec: "go" "c" "f" :=
+    if: (recv "c") then #()
+    else if: (recv "c") then "f" "c"
+    else let: "c'" := recv "c" in
+         ("go" "c" "f" ||| "go" "c'" "f");; #().
+
+Definition client_terminate : val :=
+  λ: "c", send "c" #true.
+
+Definition client_serve : val :=
+  λ: "c", send "c" #false;; send "c" #true.
+
+Definition client_duplicate : val :=
+  λ: "c",
+    send "c" #false;; send "c" #false;;
+    let: "c2" := new_chan #() in
+    send "c" (Snd "c2").
+
+Section with_Σ.
+  Context `{heapG Σ, chanG Σ, spawnG Σ}.
+
+  Lemma server_spec c (f: val) prot :
+    (∀ c', {{{ c' ↣ prot }}} f c' {{{ RET #(); True }}}) -∗
+    {{{ c ↣ (<|¡|> prot) }}} server c f {{{ RET #(); True }}}.
+  Proof.
+    iIntros "#Hfspec !>" (Φ) "Hc HΦ".
+    iLöb as "IH" forall (c Φ).
+    wp_lam.
+    rewrite {2}iProto_server_unfold.
+    wp_branch.
+    { wp_pures. by iApply "HΦ". }
+    wp_branch.
+    { wp_pures. by iApply ("Hfspec" with "Hc"). }
+    wp_recv (c') as "Hc'".
+    wp_apply (wp_par (λ w, True)%I (λ w, True)%I with "[Hc] [Hc']");
+      [ by iApply ("IH" with "Hc") | by iApply ("IH" with "Hc'") | ].
+    iIntros (v1 v2) "_ !>".
+    wp_pures. by iApply "HΦ".
+  Qed.
+
+  Lemma client_spec_terminate c prot :
+    ⊢ {{{ c ↣ <|¿|> prot }}} client_terminate c {{{ RET #(); c ↣ END }}}.
+  Proof.
+    iIntros "!>" (Φ) "Hc HΦ".
+    rewrite iProto_client_unfold.
+    wp_lam. wp_select. by iApply "HΦ".
+  Qed.
+
+  Lemma client_spec_serve c prot :
+     ⊢ {{{ c ↣ <|¿|> prot }}} client_serve c {{{ RET #(); c ↣ prot }}}.
+  Proof.
+    iIntros "!>" (Φ) "Hc HΦ".
+    rewrite iProto_client_unfold.
+    wp_lam. wp_select. wp_select. by iApply "HΦ".
+  Qed.
+
+  Lemma client_spec_duplicate c prot :
+    ⊢ {{{ c ↣ <|¿|> prot }}}
+        client_duplicate c
+      {{{ c', RET #(); c ↣ (<|¿|> prot) ∗ c' ↣ (<|¿|> prot) }}}.
+  Proof.
+    iIntros "!>" (Φ) "Hc HΦ".
+    rewrite {1}iProto_client_unfold.
+    wp_lam. wp_select. wp_select.
+    wp_apply (new_chan_spec (<|¿|> prot)%proto); [ done | ].
+    iIntros (c21 c22) "[Hc21 Hc22]".
+    wp_send with "[Hc22//]".
+    iApply "HΦ".
+    iFrame "Hc Hc21".
+  Qed.
+
+End with_Σ.
